\documentclass{ximera}
\input{../../preamble.tex}
\begin{document}
\begin{exercise} \label{c10.1.c9}
Let $A$ be an invertible $n\times n$ matrix and let $b\in\R^n$ be a column 
vector. Let $B_j$ be the $n\times n$ matrix obtained from $A$ by replacing the 
$j^{th}$ column of $A$ by the vector $b$.  Let $x=(x_1,\ldots,x_n)^t$ be the 
unique solution to $Ax=b$. Then Cramer's rule \index{Cramer's rule} states that
\begin{equation}  \label{E:cramer2}
x_j = \frac{\det(B_j)}{\det(A)}.
\end{equation}
Prove Cramer's rule.  {\bf Hint}: Let $A_j$ be the $j^{th}$ column of $A$ so
that $A_j = Ae_j$.  Show that 
\[
B_j = A (e_1|\cdots|e_{j-1}|x|e_{j+1}|\cdots|e_n).
\]
Using this product, compute the determinant of $B_j$ and verify \eqref{E:cramer2}.

\begin{solution}
\soln
Let $A$ be an invertible $n\times n$ matrix and let $b\in\R^n$ be a column 
vector. Let $B_j$ be the $n\times n$ matrix obtained from $A$ by replacing 
the $j^{th}$ column of $A$ by the vector $b$.  Let $x=(x_1,\ldots,x_n)^t$ be 
the unique solution to $Ax=b$.  We claim that
\[
x_j = \frac{\det(B_j)}{\det(A)}.
\]
Let $A_j$ be the $j^{th}$ column of $A$ so that $Ae_j=A_j$.  It follows that 
\begin{eqnarray*}
A (e_1|\cdots|e_{j-1}|x|e_{j+1}|\cdots|e_n) & = & 
(A e_1|\cdots|A e_{j-1}|A x|A e_{j+1}|\cdots|A e_n)\\
& = & (A_1|\cdots|A_{j-1}|b|A_{j+1}|\cdots|A_n) \\
& = & B_j.
\end{eqnarray*}
Therefore,
\[
\det(B_j) = \det(A)\det(e_1|\cdots|e_{j-1}|x|e_{j+1}|\cdots|e_n).
\]
We claim that 
\[
\det(e_1|\cdots|e_{j-1}|x|e_{j+1}|\cdots|e_n)=x_j,
\]
from which Cramer's rule follows.  Since $\det(C)=\det(C^t)$, we can perform
elementary column operations on $C$ while computing determinants.  In
particular, we can subtract $x_ke_k$ (for $k>j$) from the $j^{th}$ column of
\[
(e_1|\cdots|e_{j-1}|x|e_{j+1}|\cdots|e_n)
\]
without changing its determinant.  The end result is that 
\[
\det(e_1|\cdots|e_{j-1}|x|e_{j+1}|\cdots|e_n)=
\det(e_1|\cdots|e_{j-1}|y|e_{j+1}|\cdots|e_n),
\]
where $y=(x_1,\ldots,x_j,0,\ldots,0)^t$.  Since this last matrix is upper
triangular, its determinant is the product of its diagonal elements ---
which equals $x_j$. 


\end{solution}
\end{exercise}
\end{document}
