\documentclass{ximera}
\input{../../preamble.tex}


\begin{document}


\begin{exercise}   \label{YZ_7.1_Vandermonde_c} 
The $(n+1)\times (n+1)$ {\em Vandermonde matrix} \index{matrix!Vandermonde}is
\begin{equation}  \label{YZ_7.1_Vandermonde}
V_{n+1} = \Matrixc{x_1^n &x_1^{n-1}&\cdots&x_1^2&x_1&1\\
x_2^n &x_2^{n-1}&\cdots&x_2^2&x_2&1\\
\vdots&\vdots & & \vdots&\vdots &\vdots\\
x_{n+1}^n &x_{n+1}^{n-1}&\cdots&x^2_{n-1}&x_{n+1}&1\\}.
\end{equation}
Verify that
\begin{equation}  \label{YZ_7.1_Vandermonde_det}
\det(V_{n+1})=\prod_{1\le i<j\le n+1}(x_i-x_j).
\end{equation}

%\RED{(Hint: Use induction on $n$. Perform column operations similar to Exercise \ref{YZ_7.1_Vandermonde_b}.)}
\begin{solution}

\soln 

We verify \eqref{YZ_7.1_Vandermonde_det} by induction. Note that Exercise~\ref{YZ_7.1_Vandermonde_a}verifies the induction step $n = 1$.

Suppose the claim is valid for $V_n$. Subtract the second column times $x_1$ from the first column, then subtract the third column times $x_1$ from the second column, etc, until at the last step where we subtract the last column times $x_1$ from the second from the last column. By performing these operations, we get
\[
\det(V_{n+1})=
\det\Matrixc{0&0&\cdots &0&0&1\\
x_2^{n-1}(x_2-x_1) &x_2^{n-2}(x_2-x_1)&\cdots&x_2(x_2-x_1)&x_2-x_1&1\\
\vdots&\vdots & & \vdots &\vdots&\vdots\\
x_{n+1}^{n-1}(x_{n+1}-x_1) &x_{n+1}^{n-2}(x_{n+1}-x_1)&\cdots&x_{n+1}(x_{n+1}-x_1)&x_{n+1}-x_1&1}.
\]
Then by cofactor expansion \eqref{e:inductdetc} along the first row, we get
\[
\det(V_{n+1})=(-1)^{n+2}\det\Matrixc{
x_2^{n-1}(x_2-x_1) &x_2^{n-2}(x_2-x_1)&\cdots&x_2(x_2-x_1)&x_2-x_1\\
\vdots&\vdots & & \vdots &\vdots\\
x_{n+1}^{n-1}(x_{n+1}-x_1) &x_{n+1}^{n-2}(x_{n+1}-x_1)&\cdots&x_{n+1}(x_{n+1}-x_1)&x_{n+1}-x_1}.
\]
Then by taking out the common factors $(x_i-x_1)$ on the $(i-1)$-th row, we have
\begin{align*}
    \det(V_{n+1}) & =(-1)^{n+2}\prod_{i=2}^{n+1}(x_i-x_1)
    \det\Matrixc{ x_2^{n-1} & x_2^{n-2} & \cdots&x_2&1\\ \vdots&\vdots & & \vdots &\vdots\\
x_{n+1}^{n-1} &x_{n+1}^{n-2}&\cdots&x_{n+1}&1}\\ &=\prod_{i=2}^{n+1}(x_1-x_i)\det(V_n),
\end{align*}
where $V_n$ is the $n\times n$ matrix in variables $x_2,\ldots x_{n+1}$. So by induction step, $\det(V_n)=\prod_{2\le i<j\le n+1}(x_i-x_j)$. Then plug into the previous step, we find that

\[
\det(V_{n+1})=\prod_{i=2}^{n+1}(x_1-x_i)\cdot \prod_{2\le i<j\le n+1}(x_i-x_j).
\]
which is exactly the expression in $(\ref{YZ_7.1_Vandermonde})$, so we verified the claim.
\end{solution}
\end{exercise}


\end{document}

