\documentclass{ximera}

\input{../preamble.tex}

\title{A Single Differential Equation}

\begin{document}
\begin{abstract}
\end{abstract}
\maketitle

  \label{S:singlelineareqn}

Algebraic operations such as addition and multiplication are
performed on numbers while the calculus operations of
differentiation and integration are performed on functions.
Thus algebraic equations (such as $x^2=9$) are solved for
numbers ($x=\pm 3$) while differential (and integral) equations
are solved for functions.

In Chapter~\ref{lineq} we discussed how to solve systems of
linear equations, such as
\begin{eqnarray*}
x_1 + x_2 & = & 2 \\
x_1 - x_2 & = & 4
\end{eqnarray*}
for numbers
\[
x_1=3 \quad \mbox{ and } \quad x_2=-1,
\]
while in this chapter we discuss how to solve some linear systems of
differential equations for functions.

Solving a single linear equation in one unknown $x$ is a simple
task.  For example, solve
\[
2x = 4
\]
for $x=2$.  Solving a single differential equation in one unknown function
$x(t)$ is far from trivial.

\subsubsection*{Integral Calculus as a Differential Equation}
\index{integral calculus}

Mathematically, the simplest type of differential equation is:
\begin{equation} \label{e:intcalc}
\dps\frac{dx}{dt}(t) = f(t)
\end{equation}
where $f$ is some continuous function.  In words, this equation asks us
to find all functions $x(t)$ whose derivative is $f(t)$.  The fundamental
theorem of calculus tells us the answer: $x(t)$ is an antiderivative of
$f(t)$.  Thus to find all solutions, we just integrate both sides of
\eqref{e:intcalc} with respect to $t$.  Formally, using indefinite integrals, 
\begin{equation}  \label{E:integrate}
\int \frac{dx}{dt}(t)dt = \int f(t)dt + C,
\end{equation}
where $C$ is an arbitrary constant.  (It is tempting to put a constant of
integration on both sides of \eqref{E:integrate}, but two constants are not 
needed, as we can just combine both constants on the right hand side of
this equation.)   Since the indefinite integral of $dx/dt$ is just the
function $x(t)$, we have 
\begin{equation}  \label{e:intcalcsoln}
x(t) = \int f(\tau) d\tau + C.
\end{equation}
In particular, finding closed form solutions to differential equations
of the type \eqref{e:intcalc} is equivalent to finding all definite
integrals of the function $f(t)$.  Indeed, to find closed form solutions 
to differential equations like \eqref{e:intcalc} we need to know all of the 
techniques of integration from integral calculus.

We note that if $x(t)$ is a real-valued function of $t$, then we denote the 
derivative of $x$ with respect to $t$ using the following
\[
\frac{dx}{dt}\qquad \dot{x} \qquad x'
\]
all of which are standard notations for the derivative.


\subsubsection*{Initial Conditions and the Role of the Integration Constant 
$C$}

Equation \eqref{e:intcalcsoln} tells us that there are an infinite number of
solutions to the differential equation \eqref{e:intcalc}, each one
corresponding to a different choice of the constant $C$.  To understand how
to interpret the constant $C$, consider the example
\[
\dps\frac{dx}{dt}(t) = \cos t.
\]
Using \eqref{e:intcalcsoln} we see that the answer is
\[
x(t) = \int \cos\tau d\tau  + C = \sin t + C.
\]
Note that 
\[
x(0) = \sin(0) + C = C.
\]
Thus, the constant $C$ represents an {\em initial condition\/} for the  
differential equation.  We will return to the discussion of initial 
conditions several times in this chapter.


\ignore{
See Exercise~\ref{c3.1.7} for a more interesting example of this type of
differential equation.

\subsubsection*{Solutions to Differential Equations are Functions}

Consider the differential equation \index{differential equation}
\begin{equation} \label{E:verify}
\frac{dx}{dt}(t) = tx(t).
\end{equation}
Are the functions
\[
x_1(t) = t^2 \AND x_2(t) = e^{t^2/2}
\]
solutions to the differential equation \eqref{E:verify}?

To test whether or not the function $x_1(t)$ is a solution, we compute
the left and right hand sides of \eqref{E:verify}:
\begin{eqnarray*}
{\rm LHS:} & \frac{d}{dt}x_1(t) & = 2t\\
{\rm RHS:} &  tx_1(t) & = t^3.
\end{eqnarray*}
Since the left and right hand sides are unequal, the function $x_1(t)$
is not a solution to \eqref{E:verify}.

To test whether or not the function $x_2(t)$ is a solution, we again
compute the left and right hand sides of \eqref{E:verify}:
\begin{eqnarray*}
{\rm LHS:} & \frac{d}{dt}x_2(t) & = te^{t^2/2}\\
{\rm RHS:} &  tx_2(t) & = te^{t^2/2}.
\end{eqnarray*}
Since the left and right hand sides are equal, the function $x_2(t)$
is a solution to \eqref{E:verify}.

Note that we have not discussed how we knew that the function $x_2(t)$
is a solution to \eqref{E:verify}.  For the most part, the issue of how
one finds solutions to a differential equation will be discussed in later
chapters, though we do determine solutions to a very important equation next.
}

\subsubsection*{The Linear Differential Equation of Growth and Decay}

The subject of differential equations that we study begins when the function $f$
on the right hand side of \eqref{e:intcalc} depends explicitly on the
function $x$, and the simplest such differential equation is:
\[
\frac{dx}{dt}(t) = x(t).
\]
Using results from differential calculus, we can solve this equation; indeed,
we can solve the slightly more complicated equation
\begin{equation}  \label{lin1}
\frac{dx}{dt}(t) = \lambda x(t),
\end{equation}
where $\lambda\in\R$ is a constant.  The differential equation \eqref{lin1} is 
{\em linear\/} since $x(t)$ appears by itself on the right hand side.  
Moreover, \eqref{lin1} is {\em homogeneous\/} since the constant function 
$x(t)=0$ is a solution.


In words \eqref{lin1} asks: For which functions $x(t)$ is the
derivative of $x(t)$ equal to $\lambda x(t)$.  The function
\[
x(t)=e^{\lambda t}
\]
is such a function, since
\[
\frac{dx}{dt}(t) = \frac{d}{dt}e^{\lambda t} =
\lambda e^{\lambda t} = \lambda x(t).
\]
More generally, the function
\begin{equation} \label{soln1}
x(t) = K e^{\lambda t}
\end{equation}
is a solution to \eqref{lin1} for any real constant $K$.  We claim
that the functions \eqref{soln1} list all (differentiable)
functions that solve \eqref{lin1}.

To verify this claim, we let $x(t)$ be a solution to \eqref{lin1}
and show that the ratio 
\[
\frac{x(t)}{e^{\lambda t}} = x(t)e^{-\lambda t}
\]
is a constant (independent of $t$).  Using the product rule 
\index{product rule} and \eqref{lin1}, compute
\begin{eqnarray*}
\frac{d}{dt}\left[x(t)e^{-\lambda t}\right] & = &
\frac{d}{dt}\left(x(t)\right) e^{-\lambda t} +
x(t)\frac{d}{dt}\left(e^{-\lambda t}\right) \\
& = &
(\lambda x(t)) e^{-\lambda t} + x(t)(-\lambda e^{-\lambda t}) \\
& = & 0.
\end{eqnarray*}
Now recall that the only functions whose derivatives are
identically zero are the constant functions.  Thus,
\[
x(t) e^{-\lambda t} = K
\]
for some constant $K\in\R$.  Hence $x(t)$ has the form
\eqref{soln1}, as claimed.

Next, we discuss the role of the constant $K$.  We have written
the function as $x(t)$, and we have meant the reader to think of
the variable $t$ as time.  Thus $x(0)$ is the initial value of
the function $x(t)$ at time $t=0$; we say that $x(0)$ is the
{\em initial value\/}\index{initial value problem} of $x(t)$.
From \eqref{soln1} we see that
\[
x(0) = K,
\]
and that $K$ is the initial value of the solution of \eqref{lin1}.
Henceforth, we write $K$ as $x_0$ so that the notation calls
attention to the special meaning of this constant.

By deriving \eqref{soln1} we have proved:
\begin{theorem}  \label{T:singleeqn}
There is a unique solution to the {\em initial value problem\/}
\index{initial value problem}
\arraystart
\begin{equation} \label{ivp1}
\begin{array}{rcl}
\dps \frac{dx}{dt}(t) & = & \lambda x(t) \\
x(0) & = & x_0.
\end{array}
\end{equation}
\arrayfinish
That solution is
\[
x(t) = x_0e^{\lambda t}.
\]
\end{theorem}

As a consequence of Theorem~\ref{T:singleeqn} we see that there
is a qualitative difference in the behavior of solutions to
\eqref{ivp1} depending on whether $\lambda>0$ or $\lambda<0$.
Suppose that $x_0>0$.  Then
\begin{equation}  \label{explimits}
\lim_{t\to\infty} x(t) = \lim_{t\to\infty} x_0e^{\lambda t} =\left\{
\begin{array}{rl} +\infty & \quad\lambda>0 \\ 0 & \quad\lambda<0 . \end{array}
\right.
\end{equation}
When $\lambda>0$ we say that the solution has {\em exponential
growth\/}\index{exponential!growth} and when $\lambda< 0$ we say
that the solution has {\em exponential decay\/}
\index{exponential!decay}.  In either case, however, the
number $\lambda$ is called the {\em growth rate\/}\index{growth
rate}.  We can visualize this discussion by graphing the
solutions in \Matlabp.

Suppose we set $x_0=1$ and $\lambda=\pm 0.5$.  Type
\begin{verbatim}
x0 = 1;
lambda = 0.5;
t = linspace(-1,4,100);
x = x0*exp(lambda*t);
plot(t,x)
hold on
xlabel('t')
ylabel('x')
lambda = -0.5;
x = x0*exp(lambda*t);
plot(t,x)
\end{verbatim}
The result of this calculation is shown in 
Figure~\ref{graph_labelfig}.  In this way we can actually see
the difference between exponential growth ($\lambda=0.5$) and
exponential decay ($\lambda=-0.5$), as discussed in the limit in 
\eqref{explimits}.

\begin{figure}[htb]
     \centerline{%
     \includegraphics[width=3.5in]{../figures/graph1.pdf}}
     \caption{Solutions of \protect\eqref{lin1}
              for $t\in [-1,4]$, $x_0=1$ and $\lambda=\pm 0.5$.}
     \label{graph_labelfig}
\end{figure}

\ignore{
  \subsubsection*{The Inhomogeneous Linear Differential Equation}

It follows from \eqref{explimits} that solutions to the linear homogeneous
differential equation \eqref{ivp1} are either unbounded as $t\to \infty$ or 
they approach zero.  Now we consider an inhomogeneous differential 
equation and show that solutions can approach fixed values for increasing 
$t$ that are neither zero nor infinity.

As an example, consider the linear differential equation
\begin{equation} \label{E:ivp2}
\frac{dx}{dt} = -2x-6.
\end{equation}
Observe that $x(t)=0$ is not a solution of \eqref{E:ivp2} and therefore
that \eqref{E:ivp2} is {\em inhomogeneous}.  It is easy to verify, however, 
that the constant function $x(t)=-3$ is a solution.

Equation~\eqref{E:ivp2} can be solved by introducing a new function that 
transforms \eqref{E:ivp2} into a homogeneous equation.  Let
\[
y(t) = x(t) + 3,
\]
and compute
\[
\frac{dy}{dt} = \frac{dx}{dt} = -2x-6 = -2y.
\]

Using Theorem~\ref{T:singleeqn}, it follows that $y(t)$ has the form
\[
y(t) = y_0e^{-2t}.
\]
Therefore
\[
x(t) =  y_0e^{-2t}-3
\]
is a solution of \eqref{E:ivp2} for every constant $y_0$.  Moreover, 
\[
\lim_{t\to\infty} x(t) = \lim_{t\to\infty} y_0e^{-2t} -3=-3,
\]
which is neither zero nor infinity.

Any equation of the form
\begin{equation} \label{ivp2}
\frac{dx}{dt}(t)  = \lambda x(t) +\rho
\end{equation}
can be solved in a similar fashion.  Just set 
\[
y(t) = x(t) + \frac{\rho}{\lambda}.
\]
It follows from \eqref{ivp2} that
\[
\frac{dy}{dt} = \frac{dx}{dt} = \lambda x(t) +\rho =
\lambda\left( y(t)-\frac{\rho}{\lambda}\right) +\rho = \lambda y(t).
\]
Theorem~\ref{T:singleeqn} implies that $y(t) = y_0e^{\lambda t}$ for some 
constant $y_0$ and
\[
x(t) = y_0e^{\lambda t} - \frac{\rho}{\lambda}.
\]
Note that the limit of $x(t)$ as $t\to\infty$ is $-\rho/\lambda$ when 
$\lambda<0$.
}





\includeexercises


\end{document}
