\documentclass{ximera}
\input{../../preamble.tex}
\begin{document}



\noindent In Exercises~\ref{c6.1.03a} -- \ref{c6.1.03d}, consider the system of
differential equations
\begin{equation} \label{Ex.1.03}
\begin{array}{rcr}
\frac{dx}{dt}  & = & 65x+42y \\
\frac{dy}{dt}  & = & -99x-64y.
\end{array}
\end{equation}
\begin{exercise} \label{c6.1.03a}
Verify that
\[
v_1 = \vectwo{2}{-3} \AND v_2 = \vectwo{-7}{11}
\]
are eigenvectors of the coefficient matrix of \eqref{Ex.1.03} and find
the associated eigenvalues.

\begin{solution}

\ans The vector $v_1 = (2,-3)^t$ is an eigenvector with associated
eigenvalue $\lambda_1 = 2$.  The vector $v_2 = (-7,11)^t$ is an
eigenvector with associated eigenvalue $\lambda_2 = -1$.

\soln Calculate:
\[
\begin{array}{rcl}
\mattwo{65}{42}{-99}{-64}\vectwo{2}{-3} & = & \vectwo{4}{-6} =
2\vectwo{2}{-3}. \\
\mattwo{65}{42}{-99}{-64}\vectwo{-7}{11} & = & \vectwo{7}{-11} =
-1\vectwo{-7}{11}.
\end{array}
\]

\end{solution}
\end{exercise}
\begin{exercise} \label{c6.1.03b}
Find the solution to \eqref{Ex.1.03} satisfying initial conditions $X(0) =
(-14,22)^t$.

\begin{solution}
\ans The solution to \eqref{Ex.1.03} with initial
condition $X(0) = (-14,22)^t$ is
\[
X(t) = 2e^{-t}\vectwo{-7}{11}.
\]

\soln We are given two linearly independent initial conditions: $v_1$
and $v_2$.  Therefore, by Theorem~\ref{T:solvends}, 
the general solution to \eqref{Ex.1.03} with initial condition $X(0)$ is
\[
X(t) = r_1e^{2t}\vectwo{2}{-3} + r_2e^{-t}\vectwo{-7}{11}.
\]
Find $r_1$ and $r_2$ by solving:
\begin{equation}  \label{c6.1.03eq}
\vectwo{-14}{22} = r_1\vectwo{2}{-3} + r_2\vectwo{-7}{11}.
\end{equation}

\end{solution}
\end{exercise}
\begin{exercise} \label{c6.1.03c}
Find the solution to \eqref{Ex.1.03} satisfying initial conditions $X(0) =
(-3,5)^t$.

\begin{solution}
The solution with initial condition $X(0) = (-3,5)^t$ is
\[
X(t) = 2e^{2t}\vectwo{2}{-3} + e^{-t}\vectwo{-7}{11}.
\]

\soln We are given two linearly independent initial conditions: $v_1$
and $v_2$.  Therefore, by Theorem~\ref{T:solvends}, 
the general solution to \eqref{Ex.1.03} with initial condition $X(0)$ is
\[
X(t) = r_1e^{2t}\vectwo{2}{-3} + r_2e^{-t}\vectwo{-7}{11}.
\]
Find $r_1$ and $r_2$ by solving:
\begin{equation}  \label{c6.1.03eq}
\vectwo{-3}{5} = r_1\vectwo{2}{-3} + r_2\vectwo{-7}{11}.
\end{equation}

\end{solution}
\end{exercise}
\begin{exercise} \label{c6.1.03d}
Find the solution to \eqref{Ex.1.03} satisfying initial conditions $X(0) =
(9,-14)^t$.

\begin{solution}
The solution with initial condition  $X(0) = (9,-14)^t$ is
\[
X(t) = e^{2t}\vectwo{2}{-3} - e^{-t}\vectwo{-7}{11}.
\]

\soln We are given two linearly independent initial conditions: $v_1$
and $v_2$.  Therefore, by Theorem~\ref{T:solvends}, 
the general solution to \eqref{Ex.1.03} with initial condition $X(0)$ is
\[
X(t) = r_1e^{2t}\vectwo{2}{-3} + r_2e^{-t}\vectwo{-7}{11}.
\]
Find $r_1$ and $r_2$ by solving:
\begin{equation}  \label{c6.1.03eq}
\vectwo{9}{-14} = r_1\vectwo{2}{-3} + r_2\vectwo{-7}{11}.
\end{equation}



\end{solution}
\end{exercise}
\end{document}
