\documentclass{ximera}
\input{../../preamble.tex}
\begin{document}
\begin{exercise} \label{A3.7.1}
Let $A$ and $B$ be $3\times 3$ invertible matrices so that
\[
A^{-1} = \Matrix{1 & 0 & -1 \\ -1 & -1 &0 \\ 0 & 1 & -1}
\quad\text{and}\quad
B^{-1} = \Matrix{1 & 1 & 1 \\ 1 &1 &0 \\ 1 & 0 & 0}
\]
Without computing $A$ or $B$, determine the following:
\begin{enumeratea}
\item $\rank(A)$
\item The solution to 
\[
Bx=\Matrix{1 \\ 1 \\ 1}
\]
\item $(2BA)^{-1}$
\item The matrix $C$ so that $ACB+3I_3=0$.
\end{enumeratea} 



\begin{solution}
\begin{enumeratea}
\item $A$ is an invertible $3\times 3$ matrix, so $\rank(A)=3$.
\item The solution is 
\[
x = B^{-1}\Matrix{1 \\ 1 \\ 1}= \Matrix{1 & 1 & 1 \\ 1 &1 &0 \\ 1 & 0 & 0} \Matrix{1 \\ 1 \\ 1}=\Matrix{3 \\ 2 \\ 1}
\]
\item 
\[
(2BA)^{-1}=\frac{1}{2}A^{-1}B^{-1}=\frac{1}{2}
\Matrix{1 & 0 & -1 \\  -1 &-1 &0 \\  0 & 1 & -1}
\Matrix{1 & 1 & 1 \\  1 &1 &0 \\  1 & 0 & 0}
=\frac{1}{2}\Matrix{ 0 & 1 & 1 \\ -2 &-2 &-1 \\ 0 & 1 & 0}
\]
\item Recall that multiplication on the left by a matrix is not the same as multiplication on the right. We have that
\begin{align*}
ACB=-3I_3\implies&\;\;  A^{-1}ACB=-3A^{-1}I_3 &&\text{multiplying on the left by $A^{-1}$}\\
\implies & \;\; CB=-3A^{-1}\\
\implies & CBB^{-1}=-3A^{-1}B^{-1}&&\text{multiplying on the right by $B^{-1}$}\\
\implies & C=-3A^{-1}B^{-1}\\
\implies & C=-3\Matrix{ 0 & 1 & 1 \\ -2 &-2 &-1 \\ 0 & 1 & 0}
\end{align*}
\end{enumeratea}
\end{solution}
\end{exercise}
\end{document}
