\documentclass{ximera}
\input{../../preamble.tex}
\begin{document}
\begin{exercise} \label{c6.3.1}
Solve the initial value problem
\[
\begin{array}{rcr}
\dot{x} & = & 2x + 3y \\
\dot{y} & = & -3x + 2y
\end{array}
\]
where $x(0) = 1  \AND  y(0) = -2$.

\begin{solution}

\ans The solution to the initial value problem $(x(0),y(0) = (1,-2)$ for
this system is:
\[
\vectwo{x(t)}{y(t)} = \vectwo{e^{2t}(\cos(3t) - 2\sin(3t))}
{-e^{2t}(\sin(3t) + 2\cos(3t))}.
\]

\soln The system is already in Jordan Normal Form with $\sigma = 2$ and $\tau = -3$: 
\[
\begin{array}{rrr}
\dot{x} & = & \sigma x - \tau y \\
\dot{y} & = & \tau x + \sigma y \end{array}. 
\]
So, according to Table~\ref{T:3sys}
\[
\vectwo{x(t)}{y(t)} = \vectwo{e^{\sigma t}(x_0\cos(\tau t) -
y_0\sin(\tau t))}{e^{\sigma t}(x_0\sin(\tau t) +
y_0\cos(\tau t))} = \vectwo{e^{2t}(\cos(-3t) + 2\sin(-3t))}
{e^{2t}(\sin(-3t) -2\cos(-3t))}.
\]

\end{solution}
\end{exercise}
\end{document}
