\documentclass{ximera}

\input{../preamble.tex}

\title{Exact Differential Equations}

\begin{document}
\begin{abstract}
\end{abstract}
\maketitle


\label{S:exact} 

We illustrate the idea behind exact equations with the following example:
\begin{equation}  \label{eq:exactex1}
\frac{dx}{dt} = \frac{x-1}{2x-t}.
\end{equation}
Since the right hand side of \eqref{eq:exactex1} is neither of the form 
$g(x)h(t)$ nor of the form $F\left(\frac{x}{t}\right)$, it cannot be 
solved either by separation of variables or by substitution.  However, 
it is possible to determine all solutions of \eqref{eq:exactex1}, as we now 
explain.

We may rewrite \eqref{eq:exactex1} as
\begin{equation} \label{eq:exactex1a}
(2x-t)\frac{dx}{dt} =(x-1). 
\end{equation}

Suppose that $x(t)$ is a solution to \eqref{eq:exactex1} and let 
$y(t)=x(t)^2 - x(t)t + t$.  Then differentiation shows that 
\[
\dot{y} = 2x\dot{x} -\dot{x}t-x + 1 = (2x-t)\dot{x} -(x-1) =0,
\]
with the last equality coming from \eqref{eq:exactex1a}.  Thus, if $x(t)$ is a 
solution, then the function $y(t)=x(t)^2 - x(t)t + t$ is constant.  It 
follows that for each solution $x(t)$ there is a real constant $c$ such that
\begin{equation} \label{eq:xc}
x(t)^2 - x(t)t + t = c.
\end{equation}
Since \eqref{eq:xc} is quadratic in $x$, the quadratic formula determines  
two solutions for each value of $c$, namely,
\begin{equation}  \label{E:twosolns}
x_\pm(t) = \frac{t\pm\sqrt{t^2-4t+4c}}{2}.
\end{equation}
When $c=1$, the radical in \eqref{E:twosolns} is a perfect square and the 
two solutions to \eqref{eq:exactex1} are:
\[
x_+(t) = t-1 \AND x_-(t) = 1,
\]
as can readily be checked. 

\subsubsection*{Solutions Lie on Level Contours}

To derive a geometric interpretation for the identity \eqref{eq:xc},
define the function $F:\R^2\rightarrow \R$ by
\[
F(t,x) = x^2 - xt + t.
\]
A {\em level set\/}\index{level set} or 
{\em contour\/}\index{contour} of $F$ is defined to be
the set of points in the $(t,x)$-plane for which
\[
F(t,x) = c,
\]
for some real constant $c$.  Thus, \eqref{eq:xc} can now be restated
as follows: solutions $x(t)$ of the differential equation \eqref{eq:exactex1} 
lie on the level sets of $F$, since $F(t,x(t))=c$.

\subsubsection*{Drawing Contours Using \Matlab}

We use the \Matlab command {\tt contour} to illustrate how this
information helps us to visualize all the solutions.  Type
\begin{verbatim}
[t,x] = meshgrid(-1.5:0.1:1.5,-1.5:0.1:1.5);
F = x.^2 - x.*t + t;
\end{verbatim}\index{\computer!meshgrid}
After these commands the data for the surface defined by the
function $F$ in the square $[-1.5,1.5]\times [-1.5,1.5]$ is
stored in the \Matlab variable {\tt F}.  The command {\tt
contour(F)}\index{\computer!contour} allows us to display 
the level sets\index{level set} of $F$.  To have
the correct scales on the axes, type
\begin{verbatim}
contour(t,x,F)
\end{verbatim}
Now the contour\index{contour} lines --- the level sets corresponding to
different levels $c$ --- are displayed.  Moreover, we want to know to which 
levels the curves in that picture belong.  Suppose that we are interested in 
the level sets corresponding to $c\in\{ -2,-1,0,1,2,3,4,5\}$.  Then we 
obtain this information by typing
\begin{verbatim}
cs = contour(t,x,F,[-2,-1,0,1,2,3,4,5]);
clabel(cs)
xlabel('t')
ylabel('x')
\end{verbatim}\index{\computer!contour}\index{\computer!clabel}
The command {\tt clabel} allows us to label the different
contour lines\index{contour!line} by their actual level.  The desired
information is displayed in Figure~\ref{Fig:contour1}.

\begin{figure}[htb]
           \centerline{%
           \includegraphics[width=3.5in]{../figures/contour1.pdf}}
           \caption{Contour lines of $F(t,x)=x^2-xt+t$ for
          $(t,x)\in[-1.5,1.5]\times[-1.5,1.5]$.}
           \label{Fig:contour1}
\end{figure}

Note that the straight line solutions $x(t)=1$ and $x(t)=t-1$ 
correspond to the level set for $c=1$, as expected.  We can also
see from Figure~\ref{Fig:contour1} that the contour lines for
the levels $c=0,-1,-2$ have a turning point, that is, they
cannot be parameterized entirely by $t$.  

Setting $c=0$ in \eqref{E:twosolns} we find the expressions
\[
x_+(t) = \frac{1}{2}\left(t+\sqrt{t(t-4)}\right) \AND
x_-(t) = \frac{1}{2}\left(t-\sqrt{t(t-4)}\right).
\]
These functions are not real-valued for $t\in (0,4)$.  In
particular, they cannot correspond to solutions of
\eqref{eq:exactex1} for these values of $t$.  This provides
an explanation for the existence of the turning point at
$(t,x)=(0,0)$ and why the solutions $x_+(t)$ and $x_-(t)$
``collide'' at this point.

Finally, we use {\dfield}\index{\computer!dfield8} to confirm our 
theoretical discussion.  We set the values in {\sf the display window}
as in Figure~\ref{Fig:contour1} and start the computation in 
\[
(t_0,x_0)=(-0.5,x_-(-0.5))=(-0.5,-1)
\]
using the {\sf Keyboard input}.  The result --- which is in good
agreement with the contour plot\index{contour!plot} --- is shown in
Figure~\ref{Fig:contour2}.  Observe that {\dfield} will not 
stop the computation of the forward orbit on its own and one has to
use the {\sf Stop} button to stop the numerical solution.  The reason is
that the program encounters numerical difficulties approaching the turning
point $(0,0)$, since the right hand side of the differential equation is
not defined at $(0,0)$.

\begin{figure}[htb]
  \centerline{%
  \includegraphics[width=3.7in]{../figures/contour2.pdf}}
  \caption{The solution of \protect\eqref{eq:exactex1} for the
  initial value $(t_0,x_0)=(-0.5,-1)$ computed by {\dfield}.}
  \label{Fig:contour2}
\end{figure}

\subsection*{The General Definition of Exact Differential Equations}

After this motivating example, we consider the general
situation.  Suppose that we have an ordinary differential
equation of the form
\begin{equation} \label{eq:exact}
\frac{dx}{dt} = \frac{G(t,x)}{H(t,x)},
\end{equation}
where $G$ and $H$ are real-valued continuous functions.  In 
\eqref{eq:exactex1}, $G(t,x)=x-1$ and $H(t,x) = 2x-t$.
The differential equation \eqref{eq:exact} is {\em exact\/} 
\index{differential equation!exact} if
there is a function $F(t,x)$ such that
\begin{equation}  \label{e:FGH}
\frac{\partial F}{\partial t} = -G \AND
\frac{\partial F}{\partial x} =  H.
\end{equation}
Indeed, the differential equation \eqref{eq:exactex1} is exact --- just set 
$F(t,x) = x^2 - xt + t$.

Supposing that the differential equation \eqref{eq:exact} is exact, proceed as 
in the example by rewriting \eqref{eq:exact} as 
\begin{equation} \label{eq:exacta}
H(t,x)\frac{dx}{dt} - G(t,x) = 0.
\end{equation}
Let $x(t)$ be a solution to \eqref{eq:exactex1} and use the chain rule, 
\eqref{e:FGH}, and \eqref{eq:exacta} to obtain
\[
\frac{d}{dt} F(t,x(t)) = \frac{\partial F}{\partial x}\frac{dx}{dt} + 
\frac{\partial F}{\partial t} = H\frac{dx}{dt}-G = 0.
\]
Hence, solutions of \eqref{eq:exact} must lie on a level set of $F$ defined 
by $F(t,x) = c$. We have proved:

\begin{theorem} \label{thm:exact}
Assume that the differential equation \eqref{eq:exact} is exact.  Then, for any 
solution $x(t)$ of \eqref{eq:exact} with $x(t_0)=x_0$, there is a constant $c$ 
such that for all $t$ close to $t_0$, $F(t,x(t)) = c$.
\end{theorem}\index{differential equation!exact}

\subsection*{On the Existence of $F$}

In order to solve exact differential equations,
\index{differential equation!exact} we must answer two 
questions: 
\begin{itemize}
\item When does a function $F$ exist that satisfies the 
conditions in \eqref{e:FGH}?
\item If the function $F$ exists, then how can we compute it?
\end{itemize}
The following proposition, based on the equality of mixed partial derivatives, 
gives a necessary condition for having a positive answer to the first question.

\begin{proposition} \label{prop:exact}
Let $G,H:\R^2\to\R$ be differentiable functions such that
$\partial G/\partial x$ and $\partial H/\partial t$ are
continuous.  Suppose that the corresponding differential
equation \eqref{eq:exact} is exact.  Then
\begin{equation} \label{eq:Gy=Hs}
-\frac{\partial G}{\partial x} (t,x) = \frac{\partial H}{\partial
t} (t,x).
\end{equation}
\end{proposition}

\begin{proof} Using \eqref{e:FGH} we compute
\[
\frac{\partial^2 F}{\partial x\partial t} = 
-\frac{\partial G}{\partial x} (t,x) \AND 
\frac{\partial^2 F}{\partial t\partial x} = 
\frac{\partial H}{\partial t} (t,x).
\]
Since $\partial G/\partial x$ and $\partial H/\partial t$ are
continuous, equality of mixed partial derivatives holds, and
\[
-\frac{\partial G}{\partial x} = 
\frac{\partial^2 F}{\partial x\partial t} =
\frac{\partial^2 F}{\partial t\partial x} =
\frac{\partial H}{\partial t},
\]
as desired. \end{proof}

\begin{remark} \label{rmk:exact}
{\rm It can be shown that criterion \eqref{eq:Gy=Hs} is also
sufficient for the exactness of the corresponding differential
equation, if this criterion is satisfied in a region in the
$(t,x)$-plane having no holes. The proof of this result can be
found in any text on multidimensional calculus.}
\end{remark}


\subsubsection*{Two Examples}

We use two examples to illustrate the test for exactness
\index{differential equation!exact!test for}
of the underlying differential equation given by \eqref{eq:Gy=Hs}.

\noindent (a) Consider \eqref{eq:exactex1}, that is, suppose $G(t,x)=x-1$ and 
$H(t,x)=2x-t$.  Then
\[
-\frac{\partial G}{\partial x} = -1 = 
\frac{\partial H}{\partial t},
\]
and according to Remark~\ref{rmk:exact} a function $F$ with the desired 
properties may be found.

\noindent (b) Suppose that $G(t,x) = 1$ and $H(t,x) = t$.  Then 
\[
-\frac{\partial G}{\partial x} (t,x) = 0\not= 1 = 
\frac{\partial H}{\partial t} (t,x),
\]
and by Proposition~\ref{prop:exact} a function $F$ satisfying \eqref{e:FGH} 
cannot exist.

\subsection*{On the Computation of $F$}
Next, consider the second question, namely, how can $F$ be
computed when it exists.  By \eqref{e:FGH} we have
\[
\frac{\partial F}{\partial t}(t,x) = -G(t,x).
\]
Therefore, there is a differentiable function $g:\R\to\R$ such
that
\begin{equation}  \label{eq:defGamma}
F(t,x) = -\Gamma(t,x) + g(x),
\end{equation}
where 
\[
\Gamma(t,x)=\int G(\tau,x) d\tau
\]
is an indefinite integral of $G$ with respect to the variable $t$.
Condition \eqref{e:FGH} also implies that
\[
H(t,x) = \frac{\partial F}{\partial x}(t,x) =
-\frac{\partial}{\partial x}\Gamma(t,x) + g'(x),
\]
that is
\begin{equation} \label{eq:defg}
g'(x) = \frac{\partial}{\partial x}\Gamma(t,x) + H(t,x).
\end{equation}
Equations \eqref{eq:defg} and \eqref{eq:defGamma} can now be used 
to compute the function $F$ as long as the corresponding
integrations can be performed.  

Equivalently, we can first integrate the condition $F_x=H$ to obtain
\begin{equation}  \label{eq:excond}
F(t,x) = \Omega(t,x) + h(t),
\end{equation}
where $\Omega(t,x)=\int H(t,x)dx$ is an indefinite integral of $H$ with
respect to $x$.  Then \eqref{e:FGH} leads to
\[
h'(t) = -\frac{\partial}{\partial t}\Omega(t,x) - G(t,x).
\]
In practice, we prefer one way to the other depending on which
integrations are easier to perform.

\subsubsection*{Two Examples}

\noindent (a) Reconsider \eqref{eq:exactex1}, that is, suppose $G(t,x)=x-1$ and 
$H(t,x)=2x-t$.  We can choose
\[
\Gamma(t,x)=\int G(\tau,y)d\tau = tx-t,
\]
and \eqref{eq:defg} becomes
\[
g'(x) = t + H(t,x) = 2x.
\]
We can then choose $g(x)=x^2$ and, by \eqref{eq:defGamma}, obtain
\[
F(t,x) = -\Gamma(t,x) + g(x) = -tx + t + x^2.
\]

\noindent (b) Next, consider the differential equation
\begin{equation}  \label{eq:exacex2}
\frac{dx}{dt} = \frac{2t(1-x^2)-x^6}{x(2t^2+3x+6tx^4)}.
\end{equation}
In our notation
\[
G(t,x) = 2t(1-x^2)-x^6 \AND H(t,x) = x(2t^2+3x+6tx^4).
\]
Therefore, 
\[
-\frac{\partial G}{\partial x} = 4tx + 6x^5 = 
\frac{\partial H}{\partial t}.
\]
Hence the equation is exact (see Proposition~\ref{prop:exact} and 
Remark~\ref{rmk:exact}).  

It is easier to compute $\Gamma(t,x)=\int G(\tau,x) d\tau$ than 
$\Omega(t,x)=\int H(s,x)dx$.  We choose 
\[
\Gamma(t,x) = t^2(1-x^2) - tx^6,
\]
and \eqref{eq:defg} becomes
\[
g'(x) = -(2t^2 x + 6tx^5) + x(2t^2+3x+6tx^4) = 3x^2.
\]
Now we use \eqref{eq:defGamma} to obtain
\[
F(t,x) = t^2(x^2-1) + tx^6 + x^3.
\]
Solutions of the differential equation \eqref{eq:exacex2} lie on
level sets of $F$.  In particular, the solution $x(t)$
determined by the initial condition $x(2)=1$ satisfies 
\[
F(t,x)=t^2(x^2-1) + tx^6 + x^3 = 3,
\]
since $F(2,1)=3$.  To see the qualitative behavior of the
solutions\index{contour!plot} we use the following sequence 
of \Matlab commands
\begin{verbatim}
[t,x] = meshgrid(1:0.02:3,0.5:0.01:1.5);
F  = t.^2.*(x.^2-1) + t.*x.^6 + x.^3;
cs = contour(t,x,F,[0,3,6,9,12]);
clabel(cs)
hold on
plot(2,1,'o')                  
xlabel('t')
ylabel('x')
\end{verbatim}\index{\computer!meshgrid}\index{\computer!contour}
\index{\computer!hold}\index{\computer!clabel}\index{\computer!plot}
The result is shown in Figure~\ref{Fig:contour3}.  

\begin{figure}[htb]
  \centerline{%
  \includegraphics[width=3.5in]{../figures/contour3.pdf}}
  \caption{Solutions of the differential equation
\protect\eqref{eq:exacex2}
  corresponding to the levels $c=0,3,6,9,12$ in the rectangle
  $[1,3]\times [0.5,1.5]$.}
\label{Fig:contour3}
\end{figure}




\includeexercises


\end{document}
