\documentclass{ximera}
\input{../../preamble.tex}

\begin{document}

\begin{exercise} \label{YZ_3.6_assoc1}
Verify associativity of matrix multiplication $(AB)C=A(BC)$ by hand where
\[
A=\Matrix{4&-2} \quad  B=\Matrix{1\\-3} \quad C=\Matrix{0&2}.
\]

\begin{solution}
\soln Compute
\[
AB=\Matrix{10} \AND BC=\Matrix{0&2\\0&-6}.
\]
Therefore
\[
(AB)C=\Matrix{10}\Matrix{0&2}=\Matrix{0&20}.
\]
\[
A(BC)=\Matrix{4&-2}\Matrix{0&2\\0&-6}=\Matrix{0&20}.
\]
Thus $(AB)C=A(BC)$.
\end{solution}
\end{exercise}


\begin{exercise}\label{YZ_3.6_assoc2}
Verify associativity of matrix multiplication $(AB)C=A(BC)$ by hand where
\[
A=\Matrix{2&3&1\\0&-1&2} \quad B=\Matrix{0&-1\\2&3\\-2&1} \quad C=\Matrix{3&1\\0&-2}.
\]

\begin{solution}
\soln Compute
\[
AB=\Matrix{4&8\\-6&-1} \AND BC=\Matrix{0&2\\6&-4\\-6&-4}.
\]
Therefore
\[
(AB)C=\Matrix{4&8\\-6&-1}\Matrix{3&1\\0&-2}=\Matrix{12&-12\\-18&-4}.
\]
\[
A(BC)=\Matrix{2&3&1\\0&-1&2}\Matrix{0&2\\6&-4\\-6&-4}=\Matrix{12&-12\\-18&-4}.
\]
Thus $(AB)C=A(BC)$.
\end{solution}
\end{exercise}

\begin{computerExercise}\label{YZ_3.6_assoc3}
Verify associativity of matrix multiplication $(AB)C=A(BC)$ using \Matlab where
\[
A=\Matrix{5&1\\-8&-2\\7&10}\quad B=\Matrix{2&0\\3&-6} \quad C=\Matrix{4&12&-3\\-2&-5&7}
\]

\begin{solution}
\soln
Enter 
\[
\begin{array}{l}
{\tt A = [5,1;-8,-2;7,10]} \\
{\tt B = [2,0;3,-6]} \\
{\tt C = [4,12,-3;-2,-5,7]}
\end{array}
\]
to define the three matrices.  Enter 
\[
{\tt ABC1 = (A * B)*C} 
\]
and \Matlab returns the $3\times 3$ matrix
\begin{verbatim}
ABC1=

    64   186   -81
  -112  -324   150
   296   828  -552
\end{verbatim}
Next enter 
\[
{\tt ABC2 = A * ( B*C)} 
\]
and \Matlab returns the $3\times 3$ matrix
\begin{verbatim}
ABC2=

    64   186   -81
  -112  -324   150
   296   828  -552
\end{verbatim}

Observe that {\tt ABC1} = {\tt ABC2}.  Alternatively,  enter 
\[
{\tt ABC1 - ABC2} 
\]
and \Matlab returns the zero $3\times 3$ matrix.
\end{solution}

\end{computerExercise}


\end{document}