\documentclass{ximera}
\input{../../preamble.tex}

\begin{document}


In Exercise \ref{YZ_2.5_CplxCompute1}-\ref{YZ_2.5_CplxCompute4}, write the given expression 
in the form $\alpha + i\beta$ where $\alpha,\beta\in\R$:

\begin{exercise} \label{YZ_2.5_CplxCompute1}
$\frac{1-i}{1+i}$.

\begin{solution}
\ans $-i$.

\soln $\frac{1-i}{1+i}=\frac{(1-i)^2}{(1+i)(1-i)}=\frac{(1-i)^2}{1+1}=\frac{1-1-2i}{2}=\frac{-2i}{2}=-i$.
\end{solution}
\end{exercise}


\begin{exercise}\label{YZ_2.5_CplxCompute2}
$\frac{\sqrt{3}+i}{1-\sqrt{3}i}$.

\begin{solution}
\ans $i$.

\soln $\frac{\sqrt{3}+i}{1-\sqrt{3}i}=\frac{(\sqrt{3}+i)(1+\sqrt{3}i)}{(1-\sqrt{3}i)(1+\sqrt{3}i)}=\frac{\sqrt{3}-\sqrt{3}+(1+3i)}{4}=i$.
\end{solution}
\end{exercise}

\begin{exercise}\label{YZ_2.5_CplxCompute3}
$\overline{(-2+3i)}(1-2i)^2$.

\begin{solution}
\ans $-6+17i$.

\soln $\overline{(-2+3i)}(1-2i)^2=(-2-3i)[1-4+(-4)i]=(-2-3i)(-3-4i)=(2+3i)(3+4i)=6-12+(8+9)i=-6+17i$.
\end{solution}
\end{exercise}

\begin{exercise}\label{YZ_2.5_CplxCompute4}
$\frac{(5+4i)(1+i)}{3-2i}$.

\begin{solution}
\ans $\frac{-15+29i}{13}$.

\soln $\frac{(5+4i)(1+i)}{3-2i}=\frac{5-4+(4+5)i}{3-2i}=\frac{1+9i}{3-2i}=\frac{(1+9i)(3+2i)}{(3-2i)(3+2i)}=\frac{3-18+(2+27)i}{9+4}=\frac{-15+29i}{13}$.
\end{solution}
\end{exercise}

\end{document}