\documentclass{ximera}
\input{../../preamble.tex}
\begin{document}



\noindent In Exercises~\ref{c4.10A.1a} -- \ref{c4.10A.1d} find the solution
to the system of differential equations $\dot{X} = CX$ satisfying $X(0)=X_0$.
\begin{exercise}  \label{c4.10A.1a}
$C = \mattwo{1}{1}{0}{2}$ \AND $X_0 = \vectwo{1}{4}$.

\begin{solution}
\ans The solution to $\dot{X} = CX$ satisfying this
initial condition is
\[
X(t) = 4e^{2t}\vectwo{1}{1} - 3e^t\vectwo{1}{0}
= \cvectwo{4e^{2t} - 3e^t}{4e^{2t}}.
\]

\soln First, find the eigenvalues of $C$, which are the roots of the
characteristic polynomial
\[
p_C(\lambda) = \lambda^2 - \trace(C)\lambda + \det(C) =
\lambda^2 - 3\lambda + 2 = (\lambda - 2)(\lambda - 1).
\]
So the eigenvalues are: $\lambda_1 = 2$ and $\lambda_2 = 1$.
To find the eigenvector associated to each eigenvalue, solve
the equation $(C - \lambda_jI_2)v_j = 0$ for $j = 1$ and $j = 2$.  Solve
\[
\left(\mattwo{1}{1}{0}{2} - \mattwo{2}{0}{0}{2}\right)v_1 =
\mattwo{-1}{1}{0}{0}v_1 = 0
\]
to obtain $v_1 = (1,1)^t$ and solve
\[
\left(\mattwo{1}{1}{0}{2} - \mattwo{1}{0}{0}{1}\right)v_2 =
\mattwo{0}{1}{0}{1}v_2 = 0
\]
to obtain $v_2 = (1,0)^t$.  We can then write the general solution
\[
X(t) = \alpha_1e^{\lambda_1 t}v_1 + \alpha_2e^{\lambda_2 t}v_2
= \alpha_1e^{2t}\vectwo{1}{1} + \alpha_2e^t\vectwo{1}{0}.
\]
From this formula, find $\alpha_1$ and $\alpha_2$ by solving
\[
\vectwo{4}{-3} = X(0) = \alpha_1\vectwo{1}{1} + \alpha_2\vectwo{1}{0} =
\cvectwo{\alpha_1 + \alpha_2}{\alpha_1}.
\]
Solving the linear system
\[
\begin{array}{rrrrr}
\alpha_1 & + & \alpha_2 & = & 4 \\
\alpha_1 & & & = & -3
\end{array}
\]
we obtain $\alpha_1 = 4$ and $\alpha_2 = -3$ and find the
solution to the differential equation.


\end{solution}
\end{exercise}
\begin{exercise}  \label{c4.10A.1b}
$C = \mattwo{2}{-3}{0}{-1}$ \AND $X_0 = \vectwo{1}{-2}$.

\begin{solution}
\ans The solution to $\dot{X} = CX$ satisfying this
initial condition is
\[
X(t) = 3e^{2t}\vectwo{1}{0} - 2e^{-t}\vectwo{1}{1}
= \cvectwo{3e^{2t} - 2e^{-t}}{-2e^{-t}}.
\]

\soln First, find the eigenvalues of $C$, which are the roots of the
characteristic polynomial
\[
p_C(\lambda) = \lambda^2 - \trace(C)\lambda + \det(C) =
\lambda^2 - \lambda - 2 = (\lambda - 2)(\lambda + 1).
\]
So the eigenvalues are: $\lambda_1 = 2$ and $\lambda_2 = -1$.
To find the eigenvector associated to each eigenvalue, solve
the equation $(C - \lambda_jI_2)v_j = 0$ for $j = 1$ and $j = 2$.  Solve
\[
\left(\mattwo{2}{-3}{0}{-1} - \mattwo{2}{0}{0}{2}\right)v_1 =
\mattwo{0}{-3}{0}{-3}v_1 = 0
\]
to obtain $v_1 = (1,0)^t$ and solve
\[
\left(\mattwo{2}{-3}{0}{-1} + \mattwo{1}{0}{0}{1}\right)v_2 =
\mattwo{3}{-3}{0}{0}v_2 = 0
\]
to obtain $v_2 = (1,1)^t$.  We can then write the general solution
\[
X(t) = \alpha_1e^{\lambda_1 t}v_1 + \alpha_2e^{\lambda_2 t}v_2
= \alpha_1e^{2t}\vectwo{1}{0} + \alpha_2e^{-t}\vectwo{1}{1}.
\]
From this formula, find $\alpha_1$ and $\alpha_2$ by solving
\[
\vectwo{1}{-2} = X(0) = \alpha_1\vectwo{1}{0} + \alpha_2\vectwo{1}{1} =
\cvectwo{\alpha_1 + \alpha_2}{\alpha_2}.
\]
Solving the linear system
\[
\begin{array}{rrrrr}
\alpha_1 & + & \alpha_2 & = & 1 \\
& & \alpha_2 & = & -2
\end{array}
\]
we obtain $\alpha_1 = 3$ and $\alpha_2 = -2$ and find the
solution to the differential equation.


\end{solution}
\end{exercise}
\begin{exercise}  \label{c4.10A.1c}
$C = \mattwo{-3}{2}{-2}{2}$ \AND $X_0 = \vectwo{-1}{3}$.

\begin{solution}
\ans The solution to $\dot{X} = CX$ satisfying this
initial condition is
\[
X(t) = \frac{7}{3}e^t\vectwo{1}{2} - \frac{5}{3}e^{-2t}\vectwo{2}{1}
= \frac{1}{3}\cvectwo{7e^t - 10e^{-2t}}{16e^t - 5e^{-2t}}.
\]

\soln First, find the eigenvalues of $C$, which are the roots of the
characteristic polynomial
\[
p_C(\lambda) = \lambda^2 - \trace(C)\lambda + \det(C) =
\lambda^2 + \lambda - 2 = (\lambda - 1)(\lambda + 2).
\]
So the eigenvalues are: $\lambda_1 = 1$ and $\lambda_2 = -2$.
To find the eigenvector associated to each eigenvalue, solve
the equation $(C - \lambda_jI_2)v_j = 0$ for $j = 1$ and $j = 2$.  Solve
\[
\left(\mattwo{-3}{2}{-2}{2} - \mattwo{1}{0}{0}{1}\right)v_1 =
\mattwo{-4}{2}{-2}{1}v_1 = 0
\]
to obtain $v_1 = (1,2)^t$ and solve
\[
\left(\mattwo{-3}{2}{-2}{2} + \mattwo{2}{0}{0}{2}\right)v_2 =
\mattwo{-1}{2}{-2}{4}v_2 = 0
\]
to obtain $v_2 = (2,1)^t$.  We can then write the general solution
\[
X(t) = \alpha_1e^{\lambda_1 t}v_1 + \alpha_2e^{\lambda_2 t}v_2
= \alpha_1e^t\vectwo{1}{2} + \alpha_2e^{-2t}\vectwo{2}{1}.
\]
From this formula, find $\alpha_1$ and $\alpha_2$ by solving
\[
\vectwo{-1}{3} = X(0) = \alpha_1\vectwo{1}{2} + \alpha_2\vectwo{2}{1} =
\cvectwo{\alpha_1 + 2\alpha_2}{2\alpha_1 + \alpha_2}.
\]
Solving the linear system
\[
\begin{array}{rrrrr}
\alpha_1 & + & 2\alpha_2 & = & -1 \\
2\alpha_1 & + & \alpha_2 & = & 3
\end{array}
\]
we obtain $\alpha_1 = \frac{7}{3}$ and $\alpha_2 = -\frac{5}{3}$
and find the solution to the differential equation.


\end{solution}
\end{exercise}
\begin{exercise}  \label{c4.10A.1d}
$C = \mattwo{2}{1}{1}{2}$ \AND $X_0 = \vectwo{1}{2}$.

\begin{solution}
\ans The solution to $\dot{X} = CX$ satisfying this
initial condition is
\[
X(t) = \frac{3}{2}e^{3t}\vectwo{1}{1} - \frac{1}{2}e^t\vectwo{1}{-1}
= \frac{1}{2}\cvectwo{3e^{3t} - e^t}{3e^{3t} + e^t}.
\]

\soln First, find the eigenvalues of $C$, which are the roots of the
characteristic polynomial
\[
p_C(\lambda) = \lambda^2 - \trace(C)\lambda + \det(C) =
\lambda^2 - 4\lambda + 3 = (\lambda - 3)(\lambda - 1).
\]
So the eigenvalues are: $\lambda_1 = 3$ and $\lambda_2 = 1$.
To find the eigenvector associated to each eigenvalue, solve
the equation $(C - \lambda_jI_2)v_j = 0$ for $j = 1$ and $j = 2$.  Solve
\[
\left(\mattwo{2}{1}{1}{2} - \mattwo{3}{0}{0}{3}\right)v_1 =
\mattwo{-1}{1}{1}{-1}v_1 = 0
\]
to obtain $v_1 = (1,1)^t$ and solve
\[
\left(\mattwo{2}{1}{1}{2} - \mattwo{1}{0}{0}{1}\right)v_2 =
\mattwo{1}{1}{1}{1}v_2 = 0
\]
to obtain $v_2 = (1,-1)^t$.  We can then write the general solution
\[
X(t) = \alpha_1e^{\lambda_1 t}v_1 + \alpha_2e^{\lambda_2 t}v_2
= \alpha_1e^{3t}\vectwo{1}{1} + \alpha_2e^t\vectwo{1}{-1}.
\]
From this formula, find $\alpha_1$ and $\alpha_2$ by solving
\[
\vectwo{1}{2} = X(0) = \alpha_1\vectwo{1}{1} + \alpha_2\vectwo{1}{-1} =
\cvectwo{\alpha_1 + 2\alpha_2}{\alpha_1 - \alpha_2}.
\]
Solving the linear system
\[
\begin{array}{rrrrr}
\alpha_1 & + & 2\alpha_2 & = & 1 \\
\alpha_1 & - & \alpha_2 & = & 2
\end{array}
\]
we obtain $\alpha_1 = \frac{3}{2}$ and $\alpha_2 = -\frac{1}{2}$
and find the solution to the differential equation.

\end{solution}
\end{exercise}
\end{document}
