\documentclass{ximera}
\input{../../preamble.tex}
\begin{document}

\noindent {\bf Remark:}  The completion of Exercises~\ref{c6.2.7} and
\ref{c6.2.8} constitutes a proof that the infinite series definition of
the matrix exponential is a convergent series for all $n\times n$ matrices.

\begin{exercise}  \label{c6.2.7}
Let $A=(a_{ij})$ be an $n\times n$ matrix.  Define
\[
||A||_m = \max_{1\leq i\leq n} (|a_{i1}|+\cdots+|a_{in}|)
= \max_{1\leq i\leq n} \left(\sum_{j=1}^n|a_{ij}|\right).
\]
That is, to compute $||A||_m$, first sum the absolute values of the entries
in each row of $A$, and then take the maximum of these sums.  Prove that:
\[
||AB||_m \leq ||A||_m ||B||_m.
\]
{\bf Hint:} Begin by noting that
\begin{align*}
||AB||_m &=
\max_{1\leq i\leq n}\left(\sum_{j=1}^n\left|\sum_{k=1}^na_{ik}b_{kj}\right|
\right)\leq \max_{1\leq i\leq n}\left(\sum_{j=1}^n\sum_{k=1}^n\left|a_{ik}b_{kj}
           \right|\right) \\
  &= \max_{1\leq i\leq n}\left(\sum_{k=1}^n\sum_{j=1}^n
\left|a_{ik}b_{kj}\right|\right).
\end{align*}

\begin{solution}
Using the hint from the text:
\[
||AB||_m \leq \max_{1\leq i\leq n}
\left(\sum_k\sum_j\left|a_{ik}b_{kj}\right|\right) \leq
\max_{1\leq i\leq n} \left(\sum_k|a_{ik}|\sum_j|b_{kj}|\right).
\]
Then, because $\sum_j|b_{kj}|$ is the sum of the entries in the $k^{th}$
row of $B$:
\[
\max_{1\leq i\leq n}
\left(\sum_k|a_{ik}|\sum_j|b_{kj}|\right) \leq
\max_{1 \leq i \leq n}
\left(||B||_m \sum_k|a_{ik}|\right) =
||A||_m ||B||_m.
\]
Thus $||AB||_m \leq ||A||_m ||B||_m$.

\end{solution}
\end{exercise}

\begin{exercise} \label{c6.2.8}
Recall that an infinite series of real numbers
\[
c_1+c_2 +\cdots+c_N + \cdots
\]
converges absolutely if there is a constant $K$ such that for every $N$
the partial sum satisfies:
\[
|c_1| + |c_2| + \cdots + |c_N| \leq K.
\]

Let $A$ be an $n\times n$ matrix.  To prove that the matrix exponential $e^A$
is an absolutely convergent infinite series use Exercise~\ref{c6.2.7} and the
following steps.  Let $a_N$ be the $(i,j)^{th}$ entry in the matrix $A^N$
where $A^0=I_n$.
\begin{itemize}
\item[(a)]  $|a_N| \leq ||A^N||_m$.
\item[(b)]  $||A^N||_m \leq ||A||_m^N$.
\item[(c)]  $|a_0| + |a_1| + \cdots + \frac{1}{N!}|a_N| \leq e^{||A||_m}$.
\end{itemize}

\begin{solution}

(a) Let $a_{ij}$ be the $(i,j)^{th}$ entry in $n \times n$ matrix $A$. 
Then, since $|a_{ij}| \geq 0$ for all $(i,j)$,
\[ |a_{ij}| \leq |a_{i1}| + \cdots + |a_{in}| \leq
\max_i(|a_{i1}| + \cdots + |a_{in}|) = ||A||_m. \]
This statement is valid for the matrix $A^N$, so $|a_N| \leq ||A^N||_m$.

(b) To show this, we use the fact that $||A^N||_m = ||A^{N - 1}A||_m$.
According to Exercise~\ref{c6.2.7},
\[
||A^{N - 1}A||_m \leq ||A^{N - 1}||_m ||A||_m.
\]
Expanding $||A^N||_m$ in this way, we find that
\[
||A^N||_m \leq ||A||_m \cdots ||A||_m = ||A||^N_m.
\]

(c) According to our result in (a)
\[ |a_0| + |a_1| + \cdots + \frac{1}{N!}|a_N| = \sum_N
\frac{1}{N!}|a_N| \leq \sum_N \frac{1}{N!}||A^N||_m. \]
According to the result in (b)
\[ \sum_N \frac{1}{N!}||A^N||_m \leq \sum_N \frac{1}{N!}||A||^N_m. \]
We know that
\[ \sum_{N = 0}^{\infty} \frac{1}{N!}||A||^N_m = e^{||A||_m}.  \]
Therefore,
\[ \sum_N \frac{1}{N!}|a_N| \leq e^{||A||_m}, \]
so $e^A$ is absolutely convergent.





\end{solution}
\end{exercise}
\end{document}
